Work on making the initial bytecode state explicit
I'm not really sure why this needs to happen in the end, since the
initial x86 state should be what we care about, and this will be
generated from the initial x86 program. However, this initial bytecode
state will be necessary for dealing with the bytecode machine on it own.

Right now there are 2 problems.

1. I can't load the bytecode compset without breaking HOL's parser, so I
can't get the actual concrete initial bytecode state.

2. There is a cheat where we need to know that the existentially
quantified bytecode state returned from the compiler theorem is the same
as the bytecode state that we build by running bc_eval on the bytecode
program that the compiler gives us. I think this should follow from
determinism of the bytecode language.

initial/proofs/initialProgramScript.sml
@@ -1,7 +1,7 @@
 open preamble miscLib;
 open astTheory bigStepTheory initialEnvTheory interpTheory inferTheory typeSystemTheory modLangTheory conLangTheory bytecodeTheory bytecodeExtraTheory;
 open bigClockTheory untypedSafetyTheory inferSoundTheory modLangProofTheory conLangProofTheory typeSoundTheory;
-open compute_interpLib compute_inferenceLib compute_compilerLib;
+open (*compute_bytecodeLib*) compute_interpLib compute_inferenceLib compute_compilerLib;
 
 val _ = new_theory "initialProgram";
 
@@ -23,8 +23,8 @@ val _ = Hol_datatype `
                        sem_mdecls : modN set |>`;
 
 val invariant_def = Define `
-invariant se ce ⇔
-  ?genv gtagenv rd bs.
+invariant se ce bs ⇔
+  ?genv gtagenv rd.
     type_sound_invariants (NONE : (v,v) result option)
                           (convert_decls (ce.inf_mdecls, ce.inf_tdecls, ce.inf_edecls),
                            convert_menv ce.inf_tenvM,
@@ -47,13 +47,14 @@ add_to_env e prog =
     case inf_env of
       | (Success ((mdecls',tdecls',edecls'), tenvM', tenvC', tenvE'), st) =>
             SOME
-             <| inf_mdecls := mdecls' ++ e.inf_mdecls;
-                inf_tdecls := tdecls' ++ e.inf_tdecls;
-                inf_edecls := edecls' ++ e.inf_edecls;
-                inf_tenvM := tenvM' ++ e.inf_tenvM;
-                inf_tenvC := merge_tenvC tenvC' e.inf_tenvC;
-                inf_tenvE := tenvE' ++ e.inf_tenvE;
-                comp_rs := rs' |>
+             (<| inf_mdecls := mdecls' ++ e.inf_mdecls;
+                 inf_tdecls := tdecls' ++ e.inf_tdecls;
+                 inf_edecls := edecls' ++ e.inf_edecls;
+                 inf_tenvM := tenvM' ++ e.inf_tenvM;
+                 inf_tenvC := merge_tenvC tenvC' e.inf_tenvC;
+                 inf_tenvE := tenvE' ++ e.inf_tenvE;
+                 comp_rs := rs' |>,
+              code)
       | _ => NONE`;
 
 val add_to_sem_env_def = Define `
@@ -73,11 +74,13 @@ val compile_thm =
   SIMP_RULE (srw_ss()++boolSimps.DNF_ss) [AND_IMP_INTRO, evaluate_whole_prog_def] compilerProofTheory.compile_initial_prog_thm;
 
 val add_to_env_invariant_lem = Q.prove (
-`!envM envC envE cnt s tids prog cnt' s' envM' envC' envE' tids' mdecls' e e'.
+`!envM envC envE cnt s tids prog cnt' s' envM' envC' envE' tids' mdecls' e e' code bs bs'.
   closed_prog prog ∧
   evaluate_whole_prog T (envM,envC,envE) ((cnt,s),tids,set e.inf_mdecls) prog (((cnt',s'),tids',mdecls'),envC',Rval (envM',envE')) ∧
-  invariant <| sem_envM := envM; sem_envC := envC; sem_envE := envE; sem_s := s; sem_tids := tids; sem_mdecls := set e.inf_mdecls |> e ∧
-  SOME e' = add_to_env e prog
+  invariant <| sem_envM := envM; sem_envC := envC; sem_envE := envE; sem_s := s; sem_tids := tids; sem_mdecls := set e.inf_mdecls |> e bs ∧
+  SOME (e',code) = add_to_env e prog ∧
+  SOME bs' = bc_eval (bs with <| code   := bs.code ++ REVERSE code
+                               ; pc     := next_addr bs.inst_length bs.code |>)
   ⇒
   invariant <| sem_envM := envM' ++ envM;
                sem_envC := merge_envC envC' envC;
@@ -85,7 +88,7 @@ val add_to_env_invariant_lem = Q.prove (
                sem_s := s';
                sem_tids := tids';
                sem_mdecls := mdecls' |>
-            e'`,
+            e' (bs' with clock := NONE)`,
  rw [add_to_env_def, LET_THM] >>
  every_case_tac >>
  fs [] >>
@@ -116,9 +119,9 @@ val add_to_env_invariant_lem = Q.prove (
  rw [] >>
  fs [union_decls_def, convert_menv_def, typeSysPropsTheory.bvl2_append, convert_env2_def] >>
  rw [] >>
- qabbrev_tac `bs' = bs with <| clock := SOME cnt; code := bs.code++REVERSE code; pc := next_addr bs.inst_length bs.code |>` >>
+ qabbrev_tac `bs1 = bs with <| clock := SOME cnt; code := bs.code++REVERSE code; pc := next_addr bs.inst_length bs.code |>` >>
  qabbrev_tac `bc0 = bs.code` >>
- `env_rs (envM,envC,envE) ((cnt,s),tids,set e.inf_mdecls) (genv,gtagenv,rd) e.comp_rs (bs' with code := bc0)`
+ `env_rs (envM,envC,envE) ((cnt,s),tids,set e.inf_mdecls) (genv,gtagenv,rd) e.comp_rs (bs1 with code := bc0)`
              by (UNABBREV_ALL_TAC >>
                  rw [bc_state_fn_updates] >>
                  match_mp_tac compilerProofTheory.env_rs_with_bs_irr >>
@@ -126,37 +129,45 @@ val add_to_env_invariant_lem = Q.prove (
                  match_mp_tac compilerProofTheory.env_rs_change_clock >>
                  first_assum(match_exists_tac o concl) >>
                  simp[bc_state_component_equality]) >>
- `bs'.code = bc0 ++ REVERSE code`
+ `bs1.code = bc0 ++ REVERSE code`
              by (UNABBREV_ALL_TAC >>
                  rw [bc_state_fn_updates]) >>
- `IS_SOME bs'.clock`
+ `IS_SOME bs1.clock`
              by (UNABBREV_ALL_TAC >>
                  rw [bc_state_fn_updates]) >>
- `bs'.pc = next_addr bs'.inst_length bc0` by simp[Abbr`bc0`,Abbr`bs'`] >>
+ `bs1.pc = next_addr bs1.inst_length bc0` by simp[Abbr`bc0`,Abbr`bs1`] >>
  `?bs'' grd''.
-    bc_next^* bs' bs'' ∧ bc_fetch bs'' = SOME (Stop T) ∧
-    bs''.output = bs'.output ∧
+    bc_next^* bs1 bs'' ∧ bc_fetch bs'' = SOME (Stop T) ∧
+    bs''.output = bs1.output ∧
     env_rs (envM' ++ FST (envM,envC,envE),merge_envC cenv2 (FST (SND (envM,envC,envE))), envE' ++ SND (SND (envM,envC,envE))) ((cnt',s'),decls2',set q''' ∪ set e.inf_mdecls) grd'' rs' bs''`
                by metis_tac [compile_thm] >>
  fs [] >>
  pop_assum(mp_tac o MATCH_MP (REWRITE_RULE[GSYM AND_IMP_INTRO] compilerProofTheory.env_rs_change_clock)) >>
  simp[] >> disch_then(qspecl_then[`0`,`NONE`]mp_tac) >> simp[] >> strip_tac >>
- first_assum(split_pair_match o concl) >>
- first_assum(match_exists_tac o concl) >> simp[] >>
+ `bc_next^* (bs with <| code := bc0 ++ REVERSE code; pc := next_addr bs.inst_length bc0 |>) bs' ∧
+  ¬?s3. bc_next bs' s3`
+            by metis_tac [bytecodeEvalTheory.bc_eval_SOME_RTC_bc_next] >>
+ `bs' = bs''` by cheat >>
+ unabbrev_all_tac >>
+ fs [] >>
  imp_res_tac RTC_bc_next_preserves >>
- simp[Abbr`bs'`] >>
- conj_tac >- (
-   imp_res_tac compilerProofTheory.compile_initial_prog_code_labels_ok >>
-   match_mp_tac bytecodeLabelsTheory.code_labels_ok_append >> simp[] ) >>
- simp[code_executes_ok_def] >> disj1_tac >>
- metis_tac[bytecodeClockTheory.bc_fetch_with_clock,RTC_REFL]);
+ fs [] >>
+ MAP_EVERY qexists_tac [`FST grd''`, `FST (SND grd'')`, `SND (SND grd'')`] >>
+ rw []
+ >- (imp_res_tac compilerProofTheory.compile_initial_prog_code_labels_ok >>
+     match_mp_tac bytecodeLabelsTheory.code_labels_ok_append >> 
+     simp[])
+ >- (simp[code_executes_ok_def] >> disj1_tac >>
+     metis_tac[bytecodeClockTheory.bc_fetch_with_clock,RTC_REFL]));
 
 val add_to_env_invariant = Q.prove (
-`!ck envM envC envE cnt s tids prog cnt' s' envM' envC' envE' tids' mdecls' e e'.
+`!ck envM envC envE cnt s tids prog cnt' s' envM' envC' envE' tids' mdecls' e e' code bs bs'.
   closed_prog prog ∧
   evaluate_whole_prog ck (envM,envC,envE) ((cnt,s),tids,set e.inf_mdecls) prog (((cnt',s'),tids',mdecls'),envC',Rval (envM',envE')) ∧
-  invariant <| sem_envM := envM; sem_envC := envC; sem_envE := envE; sem_s := s; sem_tids := tids; sem_mdecls := set e.inf_mdecls |> e ∧ 
-  SOME e' = add_to_env e prog
+  invariant <| sem_envM := envM; sem_envC := envC; sem_envE := envE; sem_s := s; sem_tids := tids; sem_mdecls := set e.inf_mdecls |> e bs ∧ 
+  SOME (e',code) = add_to_env e prog ∧
+  SOME bs' = bc_eval (bs with <| code   := bs.code ++ REVERSE code
+                               ; pc     := next_addr bs.inst_length bs.code |>)
   ⇒ 
   invariant <| sem_envM := envM' ++ envM;
                sem_envC := merge_envC envC' envC;
@@ -164,7 +175,7 @@ val add_to_env_invariant = Q.prove (
                sem_s := s';
                sem_tids := tids';
                sem_mdecls := mdecls' |>
-            e'`,
+            e' (bs' with clock := NONE)`,
  rw [] >>
  cases_on `ck`
  >- metis_tac [add_to_env_invariant_lem] >>
@@ -173,7 +184,7 @@ val add_to_env_invariant = Q.prove (
  fs [] >>
  match_mp_tac add_to_env_invariant_lem  >>
  rw [evaluate_whole_prog_def] >>
- MAP_EVERY Q.EXISTS_TAC [`count'`,`s`, `tids`, `prog`, `0`, `e`] >>
+ MAP_EVERY Q.EXISTS_TAC [`count'`,`s`, `tids`, `prog`, `0`, `e`, `code`, `bs`] >>
  fs [no_dup_mods_def, no_dup_top_types_def]);
 
 val prim_env_def = Define `
@@ -195,39 +206,50 @@ val prim_sem_env_def = Define `
 prim_sem_env =
 add_to_sem_env <| sem_envM := []; sem_envC := ([],[]); sem_envE := []; sem_s := []; sem_tids := {}; sem_mdecls := {} |> prim_types_program`;
 
-val prim_sem_env_thm = save_thm ("prim_sem_env_thm",
-(SIMP_CONV (srw_ss()) [add_to_sem_env_def, prim_sem_env_def, prim_types_program_def]
-THENC
-computeLib.CBV_CONV compute_interpLib.the_interp_compset)
-``prim_sem_env``);
+val empty_bc_state_def = Define `
+empty_bc_state = <| 
+      stack := [];
+      code := [];
+      pc := 0;
+      refs := FEMPTY;
+      globals := [];
+      handler := 0;
+      output := "";
+      inst_length := (\x.0);
+      clock := NONE |>`;
 
-val basis_env_def = Define `
-basis_env =
-add_to_env (THE prim_env) basis_program`;
-
-val basis_sem_env_def = Define `
-basis_sem_env =
-add_to_sem_env (THE prim_sem_env) basis_program`;
+val prim_bs_def = Define `
+prim_bs = bc_eval (empty_bc_state 
+                   with <| code   := empty_bc_state.code ++ REVERSE (SND (THE prim_env))
+                         ; pc     := next_addr empty_bc_state.inst_length empty_bc_state.code |>)`
 
 val the_compiler_compset = the_compiler_compset false
 
-val prim_env_eq =
+val prim_env_eq = save_thm ("prim_env_eq",
   ``prim_env``
   |> SIMP_CONV(srw_ss())[prim_env_def,add_to_env_def,LET_THM,prim_types_program_def]
   |> CONV_RULE(computeLib.CBV_CONV the_inference_compset)
-  |> CONV_RULE(computeLib.CBV_CONV the_compiler_compset)
+  |> CONV_RULE(computeLib.CBV_CONV the_compiler_compset));
 
-val prim_sem_env_eq =
+val prim_sem_env_eq = save_thm ("prim_sem_env_eq",
   ``prim_sem_env``
   |> SIMP_CONV(srw_ss())[prim_sem_env_def,add_to_sem_env_def,prim_types_program_def]
-  |> CONV_RULE(computeLib.CBV_CONV the_interp_compset)
+  |> CONV_RULE(computeLib.CBV_CONV the_interp_compset));
+
+  (* TODO: adding the bytecode compute lib breaks the parsing of equality
+val prim_bs_eq = save_thm ("prim_bs_eq",
+  ``prim_bs``
+  |> SIMP_CONV(srw_ss())[prim_bs_def]
+  |> CONV_RULE(computeLib.CBV_CONV the_bytecode_compset));
+  *)
 
 val prim_env_inv = Q.store_thm ("prim_env_inv",
-`?se e.
-  prim_env = SOME e ∧
+`?se e code bs.
+  prim_env = SOME (e,code) ∧
   prim_sem_env = SOME se ∧
-  invariant se e`,
- simp [prim_env_eq, prim_sem_env_eq, invariant_def] >>
+  prim_bs = SOME bs ∧
+  invariant se e bs`,
+ simp [prim_env_eq, prim_sem_env_eq, invariant_def, prim_bs_def] >>
  simp[convert_decls_def,convert_menv_def,convert_env2_def,bind_var_list2_def,RIGHT_EXISTS_AND_THM] >>
  conj_tac >- (
    simp[typeSoundInvariantsTheory.type_sound_invariants_def] >>
@@ -351,6 +373,14 @@ val prim_env_inv = Q.store_thm ("prim_env_inv",
  simp[miscTheory.FEVERY_ALL_FLOOKUP] >>
  disj1_tac >>
  srw_tac[boolSimps.DNF_ss][Once RTC_CASES1]);
+
+val basis_env_def = Define `
+basis_env =
+add_to_env (FST (THE prim_env)) basis_program`;
+
+val basis_sem_env_def = Define `
+basis_sem_env =
+add_to_sem_env (THE prim_sem_env) basis_program`;
 
 val basis_env_inv = Q.store_thm ("basis_env_inv",
 `?se e.
